theories/rules_binary/rules_binary_Get.v
@@ -1,0 +1,128 @@
+From cap_machine Require Export rules_Get rules_binary_base.
+From iris.base_logic Require Export invariants gen_heap.
+From iris.program_logic Require Export weakestpre ectx_lifting.
+From iris.proofmode Require Import tactics.
+From iris.algebra Require Import frac.
+
+
+Section cap_lang_spec_rules. 
+  Context `{cfgSG Σ, MachineParameters, invG Σ}.
+  Implicit Types P Q : iProp Σ.
+  Implicit Types σ : cap_lang.state.
+  Implicit Types a b : Addr.
+  Implicit Types r : RegName.
+  Implicit Types w : Word.
+  Implicit Types reg : gmap RegName Word.
+  Implicit Types ms : gmap Addr Word.
+
+  Tactic Notation "destruct_or" ident(H) :=
+  match type of H with
+  | _ ∨ _ => destruct H as [H|H]
+  | Is_true (_ || _) => apply orb_True in H; destruct H as [H|H]
+  end.
+  Tactic Notation "destruct_or" "?" ident(H) := repeat (destruct_or H).
+  Tactic Notation "destruct_or" "!" ident(H) := hnf in H; destruct_or H; destruct_or? H.
+
+  Lemma step_Get Ep K pc_p pc_b pc_e pc_a w get_i dst src regs :
+    decodeInstrW w = get_i →
+    is_Get get_i dst src →
+
+    isCorrectPC (inr (pc_p, pc_b, pc_e, pc_a)) →
+    regs !! PC = Some (inr (pc_p, pc_b, pc_e, pc_a)) →
+    regs_of get_i ⊆ dom _ regs →
+
+    nclose specN ⊆ Ep →
+    
+    spec_ctx ∗ ⤇ fill K (Instr Executable) ∗ ▷ pc_a ↣ₐ w ∗ ▷ ([∗ map] k↦y ∈ regs, k ↣ᵣ y)
+    ={Ep}=∗ ∃ retv regs', ⤇ fill K (of_val retv) ∗ ⌜ Get_spec (decodeInstrW w) regs dst src regs' retv ⌝ ∗ pc_a ↣ₐ w ∗ ([∗ map] k↦y ∈ regs', k ↣ᵣ y).
+  Proof.
+    iIntros (Hdecode Hinstr Hvpc HPC Dregs Hnclose) "(Hinv & Hj & >Hpc_a & >Hmap)".
+    iDestruct "Hinv" as (ρ) "Hinv". rewrite /spec_inv.
+    iInv specN as ">Hinv'" "Hclose". iDestruct "Hinv'" as (e [σr σm]) "[Hown %] /=".
+    iDestruct (regspec_heap_valid_inclSepM with "Hown Hmap") as %Hregs.
+    have HPC' := regs_lookup_eq _ _ _ HPC.
+    have ? := lookup_weaken _ _ _ _ HPC Hregs.
+    iDestruct (spec_heap_valid with "[$Hown $Hpc_a]") as %Hpc_a. 
+    iDestruct (spec_expr_valid with "[$Hown $Hj]") as %Heq; subst e.
+    specialize (normal_always_step (σr,σm)) as [c [ σ2 Hstep]].
+    eapply step_exec_inv in Hstep; eauto.
+
+    specialize (indom_regs_incl _ _ _ Dregs Hregs) as Hri.
+    erewrite regs_of_is_Get in Hri; eauto.
+    destruct (Hri src) as [wsrc [H'src Hsrc]]. by set_solver+.
+    destruct (Hri dst) as [wdst [H'dst Hdst]]. by set_solver+.
+    destruct wsrc as [| (([p b] & e) & a) ] eqn:Hwsrc.
+    { (* Failure: src is not a capability *)
+      assert (c = Failed ∧ σ2 = (σr, σm)) as (-> & ->).
+      { destruct_or! Hinstr; rewrite Hinstr in Hstep; cbn in Hstep.
+        all: rewrite /RegLocate Hsrc in Hstep; inversion Hstep; auto. }
+      iFailStep Get_fail_src_noncap. }
+
+    assert ((c, σ2) = updatePC (update_reg (σr, σm) dst (inl (denote get_i (p,b,e,a))))) as HH.
+    { destruct_or! Hinstr; rewrite Hinstr /= in Hstep |- *; auto; cbn in Hstep.
+      all: destruct b, e, a; rewrite /RegLocate /update_reg Hsrc /= in Hstep |-*; auto. }
+    rewrite /update_reg /= in HH. rewrite -Hdecode in Hstep. 
+
+    destruct (incrementPC (<[ dst := inl (denote get_i (p,  b, e, a)) ]> regs))
+      as [regs'|] eqn:Hregs'; pose proof Hregs' as H'regs'; cycle 1.
+    { (* Failure: incrementing PC overflows *)
+      apply incrementPC_fail_updatePC with (m:=σm) in Hregs'.
+      eapply updatePC_fail_incl with (m':=σm) in Hregs'.
+      2: by apply lookup_insert_is_Some'; eauto.
+      2: by apply insert_mono; eauto.
+      rewrite Hdecode. clear Hdecode. simplify_pair_eq.
+      iMod ((regspec_heap_update_inSepM _ _ _ dst) with "Hown Hmap") as "[Hown Hmap]"; eauto.
+      iFailStep Get_fail_overflow_PC. } 
+
+    (* Success *)
+
+    eapply (incrementPC_success_updatePC _ σm) in Hregs'
+        as (p' & g' & b' & e' & a'' & a_pc' & HPC'' & HuPC & ->).
+    eapply updatePC_success_incl with (m':=σm) in HuPC. 2: by eapply insert_mono; eauto.
+    simplify_pair_eq. iFrame.
+    iMod ((regspec_heap_update_inSepM _ _ _ dst) with "Hown Hmap") as "[Hown Hmap]"; eauto.
+    iMod ((regspec_heap_update_inSepM _ _ _ PC) with "Hown Hmap") as "[Hown Hmap]"; eauto. 
+    iMod (exprspec_mapsto_update _ _ (fill K (Instr NextI)) with "Hown Hj") as "[Hown Hj]".
+    iExists NextIV,_. iFrame.
+    iMod ("Hclose" with "[Hown]") as "_".
+    { iNext. iExists _,_;iFrame. iPureIntro. eapply rtc_r;eauto.
+      prim_step_from_exec. }
+    iModIntro. iPureIntro. econstructor; eauto.
+  Qed.
+
+  Lemma step_Get_success E K get_i dst src pc_p pc_b pc_e pc_a w wdst csrc pc_a' :
+    decodeInstrW w = get_i →
+    is_Get get_i dst src →
+    isCorrectPC (inr (pc_p,pc_b,pc_e,pc_a)) →
+    (pc_a + 1)%a = Some pc_a' ->
+    nclose specN ⊆ E →
+    
+    spec_ctx ∗ ⤇ fill K (Instr Executable)
+             ∗ ▷ PC ↣ᵣ inr (pc_p,pc_b,pc_e,pc_a)
+             ∗ ▷ pc_a ↣ₐ w
+             ∗ ▷ src ↣ᵣ inr csrc
+             ∗ ▷ dst ↣ᵣ wdst
+    ={E}=∗ ⤇ fill K (Instr NextI)
+        ∗ PC ↣ᵣ inr (pc_p,pc_b,pc_e,pc_a')
+        ∗ pc_a ↣ₐ w
+        ∗ src ↣ᵣ inr csrc
+        ∗ dst ↣ᵣ inl (denote get_i csrc).
+  Proof.
+    iIntros (Hdecode Hinstr Hvpc Hpca' Hnlose) "(#Hown & Hj & >HPC & >Hpc_a & >Hsrc & >Hdst)".
+    iDestruct (map_of_regs_3 with "HPC Hdst Hsrc") as "[Hmap (%&%&%)]".
+    iMod (step_Get with "[$Hmap $Hj $Hown $Hpc_a]") as (retv regs') "(Hj & #Hspec & Hpc_a & Hmap)"; simplify_map_eq; eauto.
+    by erewrite regs_of_is_Get; eauto; rewrite !dom_insert; set_solver+.
+    iDestruct "Hspec" as %Hspec.
+    destruct Hspec as [| * Hfail].
+    { (* Success *)
+      iFrame. incrementPC_inv. rewrite lookup_insert_ne// lookup_insert in H6.
+      rewrite lookup_insert_ne// lookup_insert_ne// lookup_insert in H5. simplify_eq. 
+      rewrite insert_commute // insert_insert (insert_commute _ PC dst) // insert_insert.
+      iDestruct (regs_of_map_3 with "Hmap") as "(?&?&?)"; eauto; by iFrame. }
+    { (* Failure (contradiction) *)
+      destruct Hfail; eauto; rewrite lookup_insert_ne// lookup_insert_ne// lookup_insert in e; simplify_eq.
+      incrementPC_inv;[|rewrite lookup_insert_ne// lookup_insert;eauto]. congruence. }
+  Qed.
+    
+
+End cap_lang_spec_rules. 
