theories/rules_binary/rules_binary_Jmp.v
@@ -1,0 +1,98 @@
+From cap_machine Require Export rules_Jmp rules_binary_base.
+From iris.base_logic Require Export invariants gen_heap.
+From iris.program_logic Require Export weakestpre ectx_lifting.
+From iris.proofmode Require Import tactics.
+From iris.algebra Require Import frac.
+
+
+Section cap_lang_spec_rules. 
+  Context `{cfgSG Σ, MachineParameters, invG Σ}.
+  Implicit Types P Q : iProp Σ.
+  Implicit Types σ : cap_lang.state.
+  Implicit Types a b : Addr.
+  Implicit Types r : RegName.
+  Implicit Types w : Word.
+  Implicit Types reg : gmap RegName Word.
+  Implicit Types ms : gmap Addr Word.
+
+  Lemma step_jmp_success E K pc_p pc_b pc_e pc_a w r w' :
+    decodeInstrW w = Jmp r →
+    isCorrectPC (inr (pc_p,pc_b,pc_e,pc_a)) →
+    nclose specN ⊆ E →
+
+    spec_ctx ∗ ⤇ fill K (Instr Executable)
+             ∗ ▷ PC ↣ᵣ inr (pc_p,pc_b,pc_e,pc_a)
+             ∗ ▷ pc_a ↣ₐ w
+             ∗ ▷ r ↣ᵣ w'
+    ={E}=∗ ⤇ fill K (Instr NextI)
+        ∗ PC ↣ᵣ updatePcPerm w'
+        ∗ pc_a ↣ₐ w
+        ∗ r ↣ᵣ w'. 
+  Proof.
+    iIntros (Hinstr Hvpc Hnclose) "(Hinv & Hj & >HPC & >Hpc_a & >Hr)".
+    iDestruct "Hinv" as (ρ) "Hinv". rewrite /spec_inv.
+    iInv specN as ">Hinv'" "Hclose". iDestruct "Hinv'" as (e [σr σm]) "[Hown %] /=".
+    iDestruct (@spec_heap_valid with "[$Hown $Hpc_a]") as %?; auto.
+    iDestruct (@spec_regs_valid with "[$Hown $HPC]") as %?.
+    iDestruct (@spec_regs_valid with "[$Hown $Hr]") as %Hr_r0.
+    iDestruct (spec_expr_valid with "[$Hown $Hj]") as %Heq; subst e.
+    specialize (normal_always_step (σr,σm)) as [c [ σ2 Hstep]].
+    eapply step_exec_inv in Hstep; eauto.
+
+    assert (Hstep':=Hstep). 
+    rewrite /update_reg /= in Hstep. simplify_pair_eq. cbn.
+    assert ((c, σ2) = (NextI, (<[PC:=updatePcPerm w']> σr, σm))) as Heq.
+    { inversion Hstep'; simpl in *; simplify_map_eq_alt. rewrite /RegLocate Hr_r0; auto. }
+    simplify_eq.
+    iMod (@regspec_mapsto_update with "Hown HPC") as "[Hown HPC]". 
+    iMod (exprspec_mapsto_update _ _ (fill K (Instr NextI)) with "Hown Hj") as "[Hown Hj]".
+    iFrame.
+    iMod ("Hclose" with "[Hown]") as "_".
+    { iNext. iExists _,_;iFrame. iPureIntro. eapply rtc_r;eauto. 
+      exists [];eapply step_atomic with (t1:=[]) (t2:=[]);eauto. 
+      econstructor;eauto;constructor. simpl.
+      eapply step_exec_instr with (c:=(NextI, (<[PC:=updatePcPerm w']> σr, σm)));
+        rewrite /RegLocate /MemLocate;[simplify_map_eq..|];eauto. 
+    }
+    done. 
+  Qed.
+
+  Lemma wp_jmp_successPC E K pc_p pc_b pc_e pc_a w :
+    decodeInstrW w = Jmp PC →
+    isCorrectPC (inr (pc_p,pc_b,pc_e,pc_a)) →
+    nclose specN ⊆ E →
+
+    spec_ctx ∗ ⤇ fill K (Instr Executable)
+             ∗ ▷ PC ↣ᵣ inr (pc_p,pc_b,pc_e,pc_a)
+             ∗ ▷ pc_a ↣ₐ w
+    ={E}=∗  ⤇ fill K (Instr NextI)
+        ∗ PC ↣ᵣ updatePcPerm (inr (pc_p,pc_b,pc_e,pc_a))
+        ∗ pc_a ↣ₐ w.
+  Proof.
+    iIntros (Hinstr Hvpc Hnclose) "(Hinv & Hj & >HPC & >Hpc_a)".
+    iDestruct "Hinv" as (ρ) "Hinv". rewrite /spec_inv.
+    iInv specN as ">Hinv'" "Hclose". iDestruct "Hinv'" as (e [σr σm]) "[Hown %] /=".
+    iDestruct (@spec_heap_valid with "[$Hown $Hpc_a]") as %?; auto.
+    iDestruct (@spec_regs_valid with "[$Hown $HPC]") as %?.
+    iDestruct (spec_expr_valid with "[$Hown $Hj]") as %Heq; subst e.
+    specialize (normal_always_step (σr,σm)) as [c [ σ2 Hstep]].
+    eapply step_exec_inv in Hstep; eauto. assert (Hstep':=Hstep). 
+
+    rewrite /update_reg /= in Hstep. simplify_pair_eq. cbn.
+    assert ((c, σ2) = (NextI, (<[PC:=updatePcPerm (inr (pc_p, pc_b, pc_e, pc_a))]> σr, σm))) as Heq.
+    { inversion Hstep'; simpl in *; simplify_map_eq_alt. rewrite /RegLocate H4; auto. }
+    simplify_eq.
+    iMod (@regspec_mapsto_update with "Hown HPC") as "[Hown HPC]". 
+    iMod (exprspec_mapsto_update _ _ (fill K (Instr NextI)) with "Hown Hj") as "[Hown Hj]".
+    iFrame.
+    iMod ("Hclose" with "[Hown]") as "_".
+    { iNext. iExists _,_;iFrame. iPureIntro. eapply rtc_r;eauto. 
+      exists [];eapply step_atomic with (t1:=[]) (t2:=[]);eauto. 
+      econstructor;eauto;constructor. simpl.
+      eapply step_exec_instr with (c:=(NextI, (<[PC:=updatePcPerm (inr (pc_p, pc_b, pc_e, pc_a))]> σr, σm)));
+        rewrite /RegLocate /MemLocate;[simplify_map_eq..|];eauto. 
+    }
+    done. 
+  Qed.
+
+End cap_lang_spec_rules. 
