theories/rules_binary/rules_binary_Restrict.v
@@ -1,0 +1,136 @@
+From cap_machine Require Export rules_Restrict rules_binary_base.
+From iris.base_logic Require Export invariants gen_heap.
+From iris.program_logic Require Export weakestpre ectx_lifting.
+From iris.proofmode Require Import tactics.
+From iris.algebra Require Import frac.
+
+
+Section cap_lang_spec_rules. 
+  Context `{cfgSG Σ, MachineParameters, invG Σ}.
+  Implicit Types P Q : iProp Σ.
+  Implicit Types σ : cap_lang.state.
+  Implicit Types a b : Addr.
+  Implicit Types r : RegName.
+  Implicit Types w : Word.
+  Implicit Types reg : gmap RegName Word.
+  Implicit Types ms : gmap Addr Word.
+
+  Lemma step_Restrict Ep K pc_p pc_b pc_e pc_a w dst src regs :
+    decodeInstrW w = Restrict dst src ->
+    isCorrectPC (inr (pc_p, pc_b, pc_e, pc_a)) →
+    regs !! PC = Some (inr (pc_p, pc_b, pc_e, pc_a)) →
+    regs_of (Restrict dst src) ⊆ dom _ regs →
+
+    nclose specN ⊆ Ep →
+    
+    spec_ctx ∗ ⤇ fill K (Instr Executable) ∗ pc_a ↣ₐ w ∗ ([∗ map] k↦y ∈ regs, k ↣ᵣ y)
+    ={Ep}=∗ ∃ retv regs', ⌜ Restrict_spec regs dst src regs' retv ⌝ ∗ ⤇ fill K (of_val retv) ∗ pc_a ↣ₐ w ∗ ([∗ map] k↦y ∈ regs', k ↣ᵣ y).
+  Proof.
+    iIntros (Hinstr Hvpc HPC Dregs Hcls) "(#Hinv & Hj & Hpc_a & Hmap)". 
+    iDestruct "Hinv" as (ρ) "Hinv". rewrite /spec_inv.
+    iInv specN as ">Hinv'" "Hclose". iDestruct "Hinv'" as (e [σr σm]) "[Hown %] /=".
+    iDestruct (regspec_heap_valid_inclSepM with "Hown Hmap") as %Hregs.
+    have HPC' := regs_lookup_eq _ _ _ HPC.
+    have Hx := lookup_weaken _ _ _ _ HPC Hregs.
+    iDestruct (spec_heap_valid with "[$Hown $Hpc_a]") as %Hpc_a. 
+    iDestruct (spec_expr_valid with "[$Hown $Hj]") as %Heq; subst e.
+
+    specialize (normal_always_step (σr,σm)) as [c [ σ2 Hstep]].
+    eapply step_exec_inv in Hstep; eauto.
+
+    specialize (indom_regs_incl _ _ _ Dregs Hregs) as Hri.
+    unfold regs_of in Hri, Dregs. assert (Hstep':=Hstep). 
+    destruct (Hri dst) as [wdst [H'dst Hdst]]. by set_solver+.
+    destruct wdst as [| cdst]; [| destruct_cap cdst].
+    { rewrite /= /RegLocate Hdst in Hstep.
+      destruct src; inv Hstep; simplify_pair_eq.
+      all: iFailStep Restrict_fail_dst_noncap. }
+    
+    destruct (z_of_argument regs src) as [wsrc|] eqn:Hwsrc;
+      pose proof Hwsrc as H'wsrc; cycle 1.
+    { destruct src as [| r0]; cbn in Hwsrc; [ congruence |].
+      destruct (Hri r0) as [r0v [Hr'0 Hr0]]. by unfold regs_of_argument; set_solver+.
+      rewrite Hr'0 in Hwsrc. destruct r0v as [| cc]; [ congruence | destruct_cap cc].
+      assert (c = Failed ∧ σ2 = (σr, σm)) as (-> & ->).
+      { rewrite /= /RegLocate Hdst Hr0 in Hstep. by simplify_pair_eq. }
+      iFailStep Restrict_fail_src_nonz. }
+    eapply z_of_argument_Some_inv' in Hwsrc; eauto.
+
+    destruct (decide (cdst = E)).
+    { subst cdst. cbn in Hstep. rewrite /RegLocate Hdst in Hstep.
+      repeat case_match; inv Hstep; iFailStep Restrict_fail_pE. }
+    
+    destruct (PermFlowsTo (decodePerm wsrc) cdst) eqn:Hflows; cycle 1.
+    { rewrite /= /RegLocate Hdst in Hstep.
+      destruct Hwsrc as [ -> | (r0 & -> & Hr0 & Hr0') ].
+      all: rewrite ?Hr0' Hflows in Hstep.
+      all: repeat case_match; inv Hstep; iFailStep Restrict_fail_invalid_perm. }
+    
+    assert ((c, σ2) = updatePC (update_reg (σr, σm) dst (inr (decodePerm wsrc, cdst2, cdst1, cdst0)))) as HH.
+    { rewrite /= /RegLocate Hdst in Hstep.
+      destruct Hwsrc as [ -> | (r0 & -> & Hr0 & Hr0') ].
+      all: rewrite ?Hr0' Hflows in Hstep.
+      all: repeat case_match; inv Hstep; eauto; congruence. }
+    clear Hstep. rewrite /update_reg /= in HH.
+
+    destruct (incrementPC (<[ dst := inr (decodePerm wsrc, cdst2, cdst1, cdst0) ]> regs)) eqn:Hregs';
+      pose proof Hregs' as H'regs'; cycle 1.
+    { apply incrementPC_fail_updatePC with (m:=σm) in Hregs'.
+      eapply updatePC_fail_incl with (m':=σm) in Hregs'.
+      2: by apply lookup_insert_is_Some'; eauto.
+      2: by apply insert_mono; eauto.
+      simplify_pair_eq.
+      iMod ((regspec_heap_update_inSepM _ _ _ dst) with "Hown Hmap") as "[Hown Hmap]"; eauto.
+      iFailStep Restrict_fail_PC_overflow. }
+    
+    eapply (incrementPC_success_updatePC _ σm) in Hregs'
+      as (p' & g' & b' & e' & a'' & a_pc' & HPC'' & HuPC & ->).
+    eapply updatePC_success_incl with (m':=σm) in HuPC. 2: by eapply insert_mono; eauto.
+    simplify_pair_eq. iFrame.
+    iMod ((regspec_heap_update_inSepM _ _ _ dst) with "Hown Hmap") as "[Hr Hmap]"; eauto.
+    iMod ((regspec_heap_update_inSepM _ _ _ PC) with "Hr Hmap") as "[Hr Hmap]"; eauto.
+    iMod (exprspec_mapsto_update _ _ (fill K (Instr NextI)) with "Hr Hj") as "[Hown Hj]".
+    iExists NextIV,_. iFrame.
+    iMod ("Hclose" with "[Hown]") as "_".
+    { iNext. iExists _,_;iFrame. iPureIntro. eapply rtc_r;eauto.
+      prim_step_from_exec. 
+    }
+    iModIntro. iPureIntro. econstructor; eauto. Unshelve. all: try done. 
+  Qed.
+
+  Lemma step_restrict_success_z Ep K pc_p pc_b pc_e pc_a pc_a' w r1 p b e a z :
+     decodeInstrW w = Restrict r1 (inl z) →
+     isCorrectPC (inr (pc_p,pc_b,pc_e,pc_a)) →
+     (pc_a + 1)%a = Some pc_a' →
+     PermFlowsTo (decodePerm z) p = true →
+     p ≠ E →
+     nclose specN ⊆ Ep →
+    
+     spec_ctx ∗ ⤇ fill K (Instr Executable)
+              ∗ ▷ PC ↣ᵣ inr (pc_p,pc_b,pc_e,pc_a)
+              ∗ ▷ pc_a ↣ₐ w
+              ∗ ▷ r1 ↣ᵣ inr (p,b,e,a)
+     ={Ep}=∗ ⤇ fill K (Instr NextI)
+         ∗ PC ↣ᵣ inr (pc_p,pc_b,pc_e,pc_a')
+         ∗ pc_a ↣ₐ w
+         ∗ r1 ↣ᵣ inr (decodePerm z,b,e,a).
+  Proof.
+    iIntros (Hinstr Hvpc Hpca' Hflows HpE Hnclose) "(Hown & Hj & >HPC & >Hpc_a & >Hr1)".
+    iDestruct (map_of_regs_2 with "HPC Hr1") as "[Hmap %]".
+    iMod (step_Restrict with "[$Hown $Hj $Hmap $Hpc_a]") as (retv regs' Hspec) "(Hj & Hpc_a & Hregs)";
+      eauto; simplify_map_eq_alt; try rewrite lookup_insert; eauto.
+      by unfold regs_of; rewrite !dom_insert; set_solver+.
+
+    destruct Hspec as [| * Hfail].
+    { (* Success *)
+      iFrame. simpl in *. incrementPC_inv; simplify_map_eq_alt.
+      rewrite (insert_commute _ PC r1) // insert_insert
+              (insert_commute _ PC r1) // insert_insert.
+      iDestruct (regs_of_map_2 with "Hregs") as "(?&?)"; eauto; by iFrame. }
+    { (* Failure (contradiction) *)
+      destruct Hfail; simpl in *; simplify_map_eq_alt; eauto; try congruence.
+      incrementPC_inv;[|rewrite lookup_insert_ne// lookup_insert;eauto]. congruence. }
+  Qed.
+
+
+End cap_lang_spec_rules. 
